updates

generic/Zeta.Generic.Global.fst
@@ -12,14 +12,3 @@ let lemma_prefix_verifiable #vspec (gl: verifiable_log vspec) (i:nat{i <= S.leng
         with t
     in
     forall_intro aux
-
-let app_fcrs
-  (#vspec: verifier_spec)
-  (gl: verifiable_log vspec): sseq (Zeta.AppSimulate.appfn_call_res vspec.app)
-  = admit()
-
-let app_fcrs_within_ep
-  (#vspec: verifier_spec)
-  (ep: epoch)
-  (gl: verifiable_log vspec): sseq (Zeta.AppSimulate.appfn_call_res vspec.app)
-  = admit()
