generic/Zeta.GenericVerifier.fsti
@@ -313,6 +313,16 @@ let addb_prop (vspec: verifier_spec_base)
     vspec.valid vtls' ==>
     blum_add_timestamp e `ts_lt` vspec.clock vtls'
 
+let evictb_prop (vspec: verifier_spec_base)
+  = forall (e: verifier_log_entry vspec) (vtls: vspec.vtls_t).
+    {:pattern verify_step e vtls}
+    let vtls' = verify_step e vtls in
+    is_blum_evict e ==>
+    vspec.valid vtls' ==>
+    (let clock_pre = vspec.clock vtls in
+     let clock_post = vspec.clock vtls' in
+     clock_pre `ts_lt` clock_post)
+
 let verifier_log vspec = S.seq (verifier_log_entry vspec)
 
 let rec verify #vspec (tid: thread_id) (l: verifier_log vspec):
@@ -326,4 +336,4 @@ let rec verify #vspec (tid: thread_id) (l: verifier_log vspec):
 
 let verifier_spec = vspec:verifier_spec_base
     {clock_monotonic_prop vspec /\ thread_id_constant_prop vspec /\ evict_prop vspec /\ add_prop vspec /\
-     addb_prop vspec}
+     addb_prop vspec /\ evictb_prop vspec}
